\documentclass[aps,pre,notitlepage,amsmath,amssymb,amsfonts,nobibnotes,nofootinbib,superscriptaddress,onecolumn,a4paper,10pt]{revtex4-1}
\setcitestyle{authoryear,round}
\bibliographystyle{apsrev4-1}
% Use the same section numbering as ApJ
% See http://tex.stackexchange.com/questions/87131/numbering-sections
\renewcommand{\thesection}{\arabic{section}}
\renewcommand{\thesubsection}{\thesection.\arabic{subsection}}
\renewcommand{\thesubsubsection}{\thesubsection.\arabic{subsubsection}}
% Fix references
\makeatletter
\def\p@subsection{}
\def\p@subsubsection{}
\makeatother

\input{preamble}

\begin{document}

\section{Effective electromagnetic fields}
We start by a simple rederivation of the equation of motion.
The equation of motion is
\begin{equation}
  \label{eq:eom}
  \dot{\vec{v}} + 2\vec{\Omega}\times\vec{v} + \nabla\psi =
  \frac{e}{m}(\vec{E} + \vec{v}\times\vec{B}).
\end{equation}
Note that by introducing the ``effective'' electromagnetic fields
$\vec{E}_\ast$ and $\vec{B}_\ast$ via
\begin{equation}
  \frac{e}{m}\vec{E}_\ast = \frac{e}{m}\vec{E} - \nabla\psi
\end{equation}
and
\begin{equation}
  \frac{e}{m}\vec{B}_\ast = \frac{e}{m}\vec{B} + 2\vec{\Omega},
\end{equation}
we can rewrite \cref{eq:eom} as
\begin{equation}
  \dot{\vec{v}} =
  \frac{e}{m}(\vec{E}_\ast + \vec{v}\times\vec{B}_\ast).
\end{equation}

\section{Standard coordinates}
In standard coordinates the tidal potential is given by
\begin{equation}
  \label{eq:tidal-potential}
  \psi = -q\Omega^2 x^2 + \frac{1}{2}\nu^2 z^2.
\end{equation}
Assuming that in equilibrium, the \emph{horizontal} force balance is such that
the plasma is rotationally supported against gravity and the magnetic field is
frozen into the bulk flow $\vec{u}=\int\!f\vec{v}\,d^3v$ (and hence
$\vec{E}+\vec{u}\times\vec{B}=0$), we must have
\begin{equation}
  \label{eq:gravito-centrifugal-balance}
  2\vec{\Omega}\times\vec{u} + \nabla_\perp\psi = 0.
\end{equation}
From \cref{eq:tidal-potential} it follows that the horizontal gradient of
$\psi$ is
\begin{equation}
   \nabla_\perp\psi = -2q\Omega^2 x\ex.
\end{equation}
Given this, solving \cref{eq:gravito-centrifugal-balance} for $\vec{u}$ yields
\begin{equation}
  \label{eq:common-shear-flow}
  \vec{u} = Sx\ey,
\end{equation}
where
\begin{equation}
  \label{eq:rate-of-shear}
  S = -q\Omega
\end{equation}
is the rate of shear (note also that $\nabla\times\vec{u}=S\ez$).

\section{Shear along $y$}
We use the same equation of motion but the tidal potential is taken to be
given by (replacing $x$ by $y$)
\begin{equation}
  \psi = -q\Omega^2 y^2 + \frac{1}{2}\nu^2 z^2  \ .
\end{equation}
In this case, the horizontal gradient of the tidal potential is given by
\begin{equation}
   \nabla_\perp\psi = -2q\Omega^2 y\ey.
\end{equation}
Given this, \cref{eq:gravito-centrifugal-balance} is satisfied provided that
\begin{equation}
  \label{eq:common-shear-flow-2}
  \vec{u} = -Sy\ex.
\end{equation}
where the rate of shear is still given by \cref{eq:rate-of-shear}.
Note the sign changes in \cref{eq:common-shear-flow-2} compared to
\cref{eq:common-shear-flow}, but also note that we still have
\begin{equation}
  \nabla\times\vec{u} = S\ez,
\end{equation}
so that the rate of shear $S$ is the $z$-component of the background vorticity
in both coordinate systems.

\section{Implementation notes}
In the code we have (so far) $\vec{\Omega} = \Omega \ez$. In this case
\begin{equation}
  \vec{E}_\ast = \vec{E} - Sx \frac{2m\Omega}{e} \ex
\end{equation}
for the standard case and
\begin{equation}
  \vec{E}_\ast = \vec{E} - Sy \frac{2m\Omega}{e} \ey
\end{equation}
for the shear along $y$ case.

\section{Epicycles}
\begin{equation}
  \ddot{\vec{r}} + 2\vec{\Omega}\times\dot{\vec{r}} + \nabla\psi = 0.
\end{equation}
Assuming $\vec{\Omega} = \Omega \ez$
For the standard case
\begin{equation}
\nabla \psi = -2Sx\vec{\Omega}\times \ey = 2Sx\Omega \ex
\end{equation}

\begin{align}
  \ddot{x} - 2 \Omega \dot{y} + 2 S \Omega x = 0 \\
  \ddot{y} + 2 \Omega \dot{x} = 0 \ ,
\end{align}
The analytical solution in our other set of notes is reproduced here for
convenience
\begin{align}
  x(t) &= A\cos(\kappa t + \phi) + x_0, \\
  y(t) &= -\frac{2\Omega}{\kappa} A\sin(\kappa t + \phi) + y_0 + S t x_0,
\end{align}
where
\begin{equation}
  \kappa = \sqrt{2\Omega(2\Omega + S)} \ .
\end{equation}
For the new coordinate system the equations are instead
\begin{equation}
\nabla \psi = 2Sy\vec{\Omega} \times \ex = 2Sy \Omega\ey
\end{equation}

\begin{align}
  \ddot{x} - 2 \Omega \dot{y} = 0 \\
  \ddot{y} + 2 \Omega \dot{x} + 2 S \Omega y = 0 \ ,
\end{align}
We find that the analytical solution in this case is
\begin{align}
  x(t) &= +\frac{2\Omega}{\kappa} A\sin(\kappa t + \phi) + x_0 - S t y_0 \\
  y(t) &= A\cos(\kappa t + \phi) + y_0.
\end{align}
\end{document}
